Things are finally compiling again

Data/Basics.hs
@@ -1,0 +1,9 @@
+module Data.Basics where
+
+import qualified Prelude
+import qualified Data.List
+
+apply :: (a1 -> a2) -> a1 -> a2
+apply f x =
+  f x
+
