Data/IApplicative.hs
@@ -1,0 +1,35 @@
+{-# OPTIONS_GHC -cpp -fglasgow-exts #-}
+{- For Hugs, use the option -F"cpp -P -traditional" -}
+
+module Data.IApplicative where
+
+import qualified Prelude
+import qualified Data.List
+import qualified Data.IEndo as IEndo
+
+
+
+--unsafeCoerce :: a -> b
+#ifdef __GLASGOW_HASKELL__
+import qualified GHC.Base as GHC.Base
+unsafeCoerce = GHC.Base.unsafeCoerce#
+#else
+-- HUGS
+import qualified Data.IOExts as IOExts
+unsafeCoerce = IOExts.unsafeCoerce
+#endif
+
+__ :: any
+__ = Prelude.error "Logical or arity value used"
+
+data IApplicative f =
+   Build_IApplicative (IEndo.IFunctor f) (() -> () -> () -> f) (() -> () ->
+                                                               () -> () -> ()
+                                                               -> f -> f ->
+                                                               f)
+
+ipure :: (IApplicative a1) -> a3 -> a1
+ipure iApplicative x =
+  case iApplicative of {
+   Build_IApplicative is_ifunctor ipure0 iap -> unsafeCoerce ipure0 __ __ x}
+
