Data/IEndo.hs
@@ -1,0 +1,30 @@
+{-# OPTIONS_GHC -cpp -fglasgow-exts #-}
+{- For Hugs, use the option -F"cpp -P -traditional" -}
+
+module Data.IEndo where
+
+import qualified Prelude
+import qualified Data.List
+
+
+--unsafeCoerce :: a -> b
+#ifdef __GLASGOW_HASKELL__
+import qualified GHC.Base as GHC.Base
+unsafeCoerce = GHC.Base.unsafeCoerce#
+#else
+-- HUGS
+import qualified Data.IOExts as IOExts
+unsafeCoerce = IOExts.unsafeCoerce
+#endif
+
+__ :: any
+__ = Prelude.error "Logical or arity value used"
+
+type IFunctor f =
+  () -> () -> () -> () -> (() -> ()) -> f -> f
+  -- singleton inductive, whose constructor was Build_IFunctor
+  
+imap :: (IFunctor a1) -> (a4 -> a5) -> a1 -> a1
+imap iFunctor x x0 =
+  unsafeCoerce iFunctor __ __ __ __ x x0
+
