Data/IMonad.hs
@@ -1,0 +1,19 @@
+module Data.IMonad where
+
+import qualified Prelude
+import qualified Data.List
+import qualified Data.IApplicative as IApplicative
+
+
+__ :: any
+__ = Prelude.error "Logical or arity value used"
+
+data IMonad m =
+   Build_IMonad (IApplicative.IApplicative m) (() -> () -> () -> () -> m ->
+                                              m)
+
+ijoin :: (IMonad a1) -> a1 -> a1
+ijoin iMonad x =
+  case iMonad of {
+   Build_IMonad is_iapplicative ijoin0 -> ijoin0 __ __ __ __ x}
+
