Data/IState.hs
@@ -1,0 +1,57 @@
+{-# OPTIONS_GHC -cpp -fglasgow-exts #-}
+{- For Hugs, use the option -F"cpp -P -traditional" -}
+
+module Data.IState where
+
+import qualified Prelude
+import qualified Data.List
+import qualified Data.IApplicative as IApplicative
+import qualified Data.IEndo as IEndo
+import qualified Data.IMonad as IMonad
+
+
+
+--unsafeCoerce :: a -> b
+#ifdef __GLASGOW_HASKELL__
+import qualified GHC.Base as GHC.Base
+unsafeCoerce = GHC.Base.unsafeCoerce#
+#else
+-- HUGS
+import qualified Data.IOExts as IOExts
+unsafeCoerce = IOExts.unsafeCoerce
+#endif
+
+type IState i o a =
+  a -> (,) i o
+  -- singleton inductive, whose constructor was mkIState
+  
+runIState :: (IState a1 a2 a3) -> a1 -> (,) a3 a2
+runIState x =
+  x
+
+coq_IState_IFunctor :: IEndo.IFunctor (IState () () ())
+coq_IState_IFunctor _ _ _ _ f x st =
+  case runIState x st of {
+   (,) a st' -> (,) (f a) st'}
+
+iget :: IState a1 a1 a1
+iget i =
+  (,) i i
+
+coq_IState_IApplicative :: IApplicative.IApplicative (IState () () ())
+coq_IState_IApplicative =
+  IApplicative.Build_IApplicative coq_IState_IFunctor (\_ _ x st -> (,) x st)
+    (\_ _ _ _ _ f x st ->
+    case runIState f st of {
+     (,) f' st' ->
+      case runIState x st' of {
+       (,) x' st'' -> (,) (unsafeCoerce f' x') st''}})
+
+coq_IState_IMonad :: IMonad.IMonad (IState () () ())
+coq_IState_IMonad =
+  IMonad.Build_IMonad coq_IState_IApplicative (\_ _ _ _ x st ->
+    case runIState x st of {
+     (,) y st' ->
+      case runIState (unsafeCoerce y) st' of {
+       (,) a st'' -> (,) a st''}})
+
