Data/Lib.hs
@@ -12,12 +12,6 @@ uncurry_sig :: (a1 -> () -> a2) -> a1 -> a2
 uncurry_sig f p =
   f p __
 
-fromMaybe :: a1 -> (Prelude.Maybe a1) -> a1
-fromMaybe d mx =
-  case mx of {
-   Prelude.Just x -> x;
-   Prelude.Nothing -> d}
-
 exist_in_cons :: a1 -> ([] a1) -> a1 -> a1
 exist_in_cons a l x =
   case l of {
